src/Ast/AstValid.dfy
@@ -1,0 +1,36 @@
+module AstValid {
+  import Ast
+  import StaticConsistency
+
+  export
+    reveals Program, Procedure, StmtSeq, Stmt, AExprSeq, AExpr
+    provides Ast, StaticConsistency
+
+  predicate Program(b3: Ast.Program)
+    reads b3.procedures, b3.functions
+  {
+    b3.WellFormed() && StaticConsistency.Consistent(b3)
+  }
+
+  predicate Procedure(proc: Ast.Procedure)
+    reads proc
+  {
+    proc.WellFormed() && StaticConsistency.ConsistentProc(proc)
+  }
+
+  predicate StmtSeq(stmts: seq<Ast.Stmt>) {
+    forall stmt <- stmts :: Stmt(stmt)
+  }
+
+  predicate Stmt(stmt: Ast.Stmt) {
+    stmt.WellFormed() && StaticConsistency.ConsistentStmt(stmt)
+  }
+
+  predicate AExprSeq(aexprs: seq<Ast.AExpr>) {
+    forall ae <- aexprs :: AExpr(ae)
+  }
+
+  predicate AExpr(ae: Ast.AExpr) {
+    ae.WellFormed() && StaticConsistency.ConsistentAExpr(ae)
+  }
+}
