src/Verifier/SpecConversions.dfy
@@ -1,0 +1,69 @@
+module SpecConversions {
+  import opened Basics
+  import opened Ast
+  import AstValid
+  import StaticConsistency
+
+  export
+    provides ToCheck, ToLearn, Learn
+    provides Basics, Ast, AstValid, StaticConsistency
+
+  function ToCheck(spec: seq<AExpr>): (stmts: seq<Stmt>)
+    requires AstValid.AExprSeq(spec)
+    ensures AstValid.StmtSeq(stmts)
+  {
+    if spec == [] then
+      []
+    else
+      var ae, rest := spec[0], ToCheck(spec[1..]);
+      assert AstValid.AExpr(ae);
+      match ae
+      case AExpr(cond) =>
+        [Check(cond)] + rest
+      case AAssertion(s) =>
+        var L := Learn(s);
+        [Assume(L)] + rest
+  }
+
+  function ToLearn(spec: seq<AExpr>): (stmts: seq<Stmt>)
+    requires AstValid.AExprSeq(spec)
+    ensures AstValid.StmtSeq(stmts)
+  {
+    if spec == [] then
+      []
+    else
+      var ae, rest := spec[0], ToCheck(spec[1..]);
+      assert AstValid.AExpr(ae);
+      match ae
+      case AExpr(cond) =>
+        [Assume(cond)] + rest
+      case AAssertion(s) =>
+        var L := Learn(s);
+        [Assume(L)] + rest
+  }
+
+  function Learn(stmt: Stmt): Expr
+    requires AstValid.Stmt(stmt) && !StaticConsistency.ContainsNonAssertions(stmt)
+    ensures Learn(stmt).WellFormed()
+  {
+    match stmt
+    case VarDecl(v, Some(rhs), body) =>
+      Expr.CreateLet(v, rhs, Learn(body))
+    case Block(stmts) =>
+      var ll := SeqMap(stmts, (s: Stmt) requires s in stmts => Learn(s));
+      Expr.CreateBigAnd(ll)
+    case Check(_) =>
+      Expr.CreateTrue()
+    case Assume(e) =>
+      e
+    case Assert(e) =>
+      e
+    case AForall(v, body) =>
+      Expr.CreateForall(v, Learn(body))
+    case Choose(branches) =>
+      var ll := SeqMap(branches, (s: Stmt) requires s in branches => Learn(s));
+      Expr.CreateBigOr(ll)
+    case Probe(_) =>
+      Expr.CreateTrue()
+  }
+}
